src/Rupicola/Lib/SepReification.v
@@ -1,0 +1,163 @@
+From coqutil Require Import
+     Decidable Map.Interface.
+From bedrock2 Require Import
+     Lift1Prop Map.Separation.
+From Coq Require Import
+     Classes.Morphisms List.
+From Rupicola Require Import Core.
+
+Import ListNotations.
+Open Scope list_scope.
+
+Module SepReif.
+Section Reification.
+  Context {key value} {map : map.map key value} {map_ok : map.ok map}.
+  Context {key_eqb: key -> key -> bool} {key_eq_dec: EqDecider key_eqb}.
+
+  Notation unseps := (unseps (map := map)).
+
+  Inductive expr :=
+    | Pred (p: map -> Prop)
+    | Sep (s1 s2: expr)
+    | Unsep (s1 s2: expr).
+
+  Fixpoint denote (e: expr) : map -> Prop :=
+    match e with
+    | Pred p => p
+    | Sep s1 s2 => sep (denote s1) (denote s2)
+    | Unsep s1 s2 => unsep (denote s1) (denote s2)
+    end.
+
+  Fixpoint unsep_normal_form' (e: expr) : list expr :=
+    match e with
+    | Pred p => [Pred p]
+    | Sep s1 s2 =>
+      map2 Sep (product (unsep_normal_form' s1)
+                        (unsep_normal_form' s2))
+    | Unsep s1 s2 =>
+      unsep_normal_form' s1 ++ unsep_normal_form' s2
+    end.
+
+  Fixpoint Unseps (es: list expr) :=
+    match es with
+    | [] => Pred (pure True)
+    | [e] => e
+    | e :: es => Unsep e (Unseps es)
+    end.
+
+  Definition unsep_normal_form (e: expr) :=
+    Unseps (unsep_normal_form' e).
+
+  Lemma denote_Unseps :
+    forall es, denote (Unseps es) = unseps (List.map denote es).
+  Proof.
+    induction es as [| e [|] IHes]; simpl in *; congruence.
+  Qed.
+
+  Lemma product_map {A B A' B'} (fA: A -> A') (fB: B -> B'):
+    forall As Bs,
+      product (List.map fA As) (List.map fB Bs) =
+      map2 (fun a b => (fA a, fB b)) (product As Bs).
+  Proof.
+    unfold map2, product; intros.
+    rewrite !flat_map_concat_map, !concat_map, !map_map.
+    f_equal; apply map_ext; intros; rewrite !map_map.
+    reflexivity.
+  Qed.
+
+  Lemma denote_map2_Sep :
+    forall es1 es2,
+      List.map denote (map2 Sep (product es1 es2)) =
+      map2 sep (product (List.map denote es1)
+                        (List.map denote es2)).
+  Proof.
+    intros.
+    rewrite product_map, map2_map2, map_map2.
+    reflexivity.
+  Qed.
+
+  Lemma unsep_normal_form_sound :
+    forall e, impl1 (denote e) (denote (unsep_normal_form e)).
+  Proof.
+    unfold unsep_normal_form; induction e; simpl; intros;
+      rewrite ?IHe1, ?IHe2,
+        ?denote_Unseps, ?denote_map2_Sep,
+        ?unseps_distr_sep, ?map_app,
+        ?unseps_app in *; reflexivity.
+  Qed.
+
+  Fixpoint denote_unseps_as_conj (es: list expr) m :=
+    match es with
+    | [] => True
+    | [e] => denote e m
+    | e :: es => denote e m /\ denote_unseps_as_conj es m
+    end.
+
+  Lemma unsep_normal_form_sound' e m:
+    denote e m ->
+    denote_unseps_as_conj (unsep_normal_form' e) m.
+  Proof.
+    intros H%unsep_normal_form_sound;
+      unfold unsep_normal_form in H;
+      rewrite denote_Unseps in H.
+    induction (unsep_normal_form' e) as [| p [|] IHps];
+      simpl in *; unfold unsep in *; auto.
+    intuition.
+  Qed.
+End Reification.
+
+  Ltac reify e :=
+    let rec loop e :=
+        match e with
+        | sep ?s1 ?s2 =>
+          let ur1 := loop s1 in let ur2 := loop s2 in uconstr:(Sep ur1 ur2)
+        | unsep ?s1 ?s2 =>
+          let ur1 := loop s1 in let ur2 := loop s2 in uconstr:(Unsep ur1 ur2)
+        | ?p => uconstr:(Pred p)
+        end in
+    let ur := loop e in
+    type_term ur.
+End SepReif.
+
+Module Tactics.
+  Ltac decompose_one_unsep H :=
+    unfold unsep in H; cbv beta in H; decompose [and] H; clear H.
+
+  Ltac decompose_all_unsep :=
+    repeat match goal with
+           | [ H: (unsep _ _) ?m |- _ ] => decompose_one_unsep H
+           end.
+
+  Ltac decompose_relevant_unsep :=
+    repeat match goal with
+           | [ H: (unsep _ _) ?m |- (sep _ _) ?m ] => decompose_one_unsep H
+           end.
+
+  Ltac normalize_relevant_sep :=
+    match goal with
+    | [ H: ?P ?m |- (sep _ _) ?m ] =>
+      lazymatch P with
+      | context[unsep] =>
+        lazymatch type of H with
+        | P m => fail "No progress"
+        | _ => idtac
+        end
+      end
+    | _ => fail "No hypothesis to normalize"
+    end.
+
+  Ltac normalize_decompose_relevant_sep :=
+    match goal with
+    | [ H: ?P ?m |- (sep _ _) ?m ] =>
+      lazymatch P with
+      | context[unsep] =>
+        let r := SepReif.reify P in
+        change P with (SepReif.denote r) in H;
+        apply SepReif.unsep_normal_form_sound' in H;
+        simpl in H; decompose [and] H; clear H
+      end
+    | _ => fail "No hypothesis to normalize"
+    end.
+End Tactics.
+
+Export Tactics.
